src/tactic/core.lean
@@ -4,6 +4,7 @@ Released under Apache 2.0 license as described in the file LICENSE.
 Authors: Mario Carneiro, Simon Hudon, Scott Morrison, Keeley Hoek
 -/
 import data.dlist.basic
+import logic.function.basic
 import control.basic
 import meta.expr
 import meta.rb_map
@@ -524,7 +525,7 @@ meta def revert_deps (e : expr) : tactic ℕ := do
 meta def is_local_def (e : expr) : tactic unit :=
 retrieve $ do revert e, expr.elet _ _ _ _ ← target, skip
 
-/-- like `split_on_p p xs`, `partition_local_deps_aux vs xs acc` searches for matches in `xs` 
+/-- like `split_on_p p xs`, `partition_local_deps_aux vs xs acc` searches for matches in `xs`
 (using membership to `vs` instead of a predicate) and breaks `xs` when matches are found.
 whereas `split_on_p p xs` removes the matches, `partition_local_deps_aux vs xs acc` includes
 them in the following partition. Also, `partition_local_deps_aux vs xs acc` discards the partition
@@ -1156,15 +1157,32 @@ meta def dependent_pose_core (l : list (expr × expr)) : tactic unit := do
 /-- Like `mk_local_pis` but translating into weak head normal form before checking if it is a `Π`.
 -/
 meta def mk_local_pis_whnf (e : expr) (md := semireducible) : tactic (list expr × expr) := do
-(expr.pi n bi d b) ← whnf e md | return ([], e),
-p ← mk_local' n bi d,
-(ps, r) ← mk_local_pis (expr.instantiate_var b p),
-return ((p :: ps), r)
+  expr.pi n bi d b ← whnf e md | return ([], e),
+  p ← mk_local' n bi d,
+  (ps, r) ← mk_local_pis (expr.instantiate_var b p),
+  return ((p :: ps), r)
 
-/-- Changes `(h : ∀xs, ∃a:α, p a) ⊢ g` to `(d : ∀xs, a) (s : ∀xs, p (d xs) ⊢ g` and
- `(h : ∀xs, p xs ∧ q xs) ⊢ g` to `(d : ∀xs, p xs) (s : ∀xs, q xs) ⊢ g` 
- `choose1` returns the second local constant it introduces. -/
-meta def choose1 (h : expr) (data : name) (spec : name) : tactic expr := do
+meta def mk_else_default (u : level) (α inh p : expr) :
+  list expr → expr × expr → tactic (expr × expr)
+| [] (val, spec) := pure (val, spec)
+| (e :: ctxt) (val, spec) := do
+  (val, spec) ← mk_else_default ctxt (val, spec),
+  t ← infer_type e,
+  b ← is_prop t,
+  pure $ if b then
+    let val' := expr.bind_lambda val e in
+    (expr.const ``function.else_default [level.zero, u] t α inh val',
+     expr.const ``function.else_default_spec [u] t α inh p val' e spec)
+  else (val, spec)
+
+/-- Changes `(h : ∀xs, ∃a:α, p a) ⊢ g` to `(d : ∀xs, a) (s : ∀xs, p (d xs)) ⊢ g` and
+`(h : ∀xs, p xs ∧ q xs) ⊢ g` to `(d : ∀xs, p xs) (s : ∀xs, q xs) ⊢ g`
+`choose1` returns the second local constant it introduces.
+
+If `nondep` is true and `α` is inhabited, then it will remove the dependency of `d` on
+all propositional assumptions in `xs`. For example if `ys` are propositions then
+`(h : ∀xs ys, ∃a:α, p a) ⊢ g` becomes `(d : ∀xs, a) (s : ∀xs ys, p (d xs)) ⊢ g`. -/
+meta def choose1 (nondep : bool) (h : expr) (data : name) (spec : name) : tactic expr := do
   t ← infer_type h,
   (ctxt, t) ← mk_local_pis_whnf t,
   t ← whnf t transparency.all,
@@ -1172,12 +1190,19 @@ meta def choose1 (h : expr) (data : name) (spec : name) : tactic expr := do
   | `(@Exists %%α %%p) := do
     α_t ← infer_type α,
     expr.sort u ← whnf α_t transparency.all,
-    value ← mk_local_def data (α.pis ctxt),
-    t' ← head_beta (p.app (value.mk_app ctxt)),
+    (ctxt', inh) ← (do
+        guard nondep,
+        inh ← mk_instance (expr.const ``inhabited [u] α),
+        ctxt' ← ctxt.mfilter (λ e, bnot <$> is_proof e),
+        pure (ctxt', some inh)) <|>
+      pure (ctxt, none),
+    value ← mk_local_def data (α.pis ctxt'),
+    t' ← head_beta (p.app (value.mk_app ctxt')),
     spec ← mk_local_def spec (t'.pis ctxt),
-    dependent_pose_core [
-      (value, ((((expr.const `classical.some [u]).app α).app p).app (h.mk_app ctxt)).lambdas ctxt),
-      (spec, ((((expr.const `classical.some_spec [u]).app α).app p).app (h.mk_app ctxt)).lambdas ctxt)],
+    (value_proof, spec_proof) ← inh.elim pure (λ inh, mk_else_default u α inh p ctxt)
+      (expr.const ``classical.some [u] α p (h.mk_app ctxt),
+       expr.const ``classical.some_spec [u] α p (h.mk_app ctxt)),
+    dependent_pose_core [(value, value_proof.lambdas ctxt'), (spec, spec_proof.lambdas ctxt)],
     try (tactic.clear h),
     intro1,
     intro1
@@ -1190,8 +1215,9 @@ meta def choose1 (h : expr) (data : name) (spec : name) : tactic expr := do
   end
 
 /-- Changes `(h : ∀xs, ∃as, p as ∧ q as) ⊢ g` to a list of functions `as`,
-and a final hypothesis on `p as` and `q as`. -/
-meta def choose : expr → list name → tactic unit
+and a final hypothesis on `p as` and `q as`. If `nondep` is true then the functions will
+be made to not depend on propositional arguments, when possible. -/
+meta def choose (nondep : bool) : expr → list name → tactic unit
 | h [] := fail "expect list of variables"
 | h [n] := do
   cnt ← revert h,
@@ -1199,7 +1225,7 @@ meta def choose : expr → list name → tactic unit
   intron (cnt - 1),
   return ()
 | h (n::ns) := do
-  v ← get_unused_name >>= choose1 h n,
+  v ← get_unused_name >>= choose1 nondep h n,
   choose v ns
 
 /--
